assignment1

lecture03.dfy
@@ -1,28 +1,167 @@
-// include "lecture02.dfy"
+/*
 
-// predicate isSubset(A: set, B: set)
-// {
-//     forall n :: n in A ==> n in B // for all objects n in set A, they also objects in set B. same as "A <= B"
-// }
+lecture 3: first proofs (of lemmas)
 
-// lemma intersectionIsSubsetofBoth(A: set, B: set, C: set) // Lemma - טענה, Name, Parameters
-//     requires pre: C == setIntersection(A, B) // == A*B, Requiers for parameters
-//     ensures isSubset (C, A) // C <= A
-//     ensures isSubset (C, B) // C <= B
-// { // הוכחת נכונות
-//   // Post 1:
-//     assert isSubset(C,A) by {
-//             forall n | n in C ensures n in A {
-//                 assert L1; n in C; // we know this
-//                 assert n in A && n in B; {reveal pre,L1; }// by the deffinition of setIntersection
-//                 assert n in A; // by { reveal pre; } this is what we need to prove
-//             }
-//         }
-// }
+- predicates
+- using Dafny's "forall ... ensures" construct
+- giving labels to assertions and "requires" clauses, and referring to them with "reveal"
+  (to justify correctness of the next assertion)
+- transitivity of the set inclusion relation
+- some further properties of sets and their operations
+- a first look on the negation of a quantifier
 
-lemma andMeansBoth(P: bool, Q: bool) // Lemma - טענה, Name, Parameters with DataTypes
-    ensures P && Q ==> P // ensure that if P and Q = True, then P = True. For ex. P || Q ==> P: It's wrong cause if only Q = True, this is NOT ensures that P = True. 
-    ensures P && Q ==> Q // ensure that if P and Q = True, then Q = True
+*/
+
+include "lecture02.dfy"
+
+// but first, one more truth table: logical equivalence (bidirectional implication)
+/*
+
+The truth table of equivalence (<-->, in Dafny <==>):
+
+ P  Q  (P <--> Q)
+ F  F  T
+ F  T  F
+ T  F  F
+ T  T  T
+
+ */
+
+//function IsSubset(A: set, B: set): bool
+predicate IsSubset(A: set, B: set) // <=
+{
+	forall n :: n in A ==> n in B // same as the next line
+	//forall n :: if n in A then n in B else true // same as "A <= B"
+}
+
+lemma IntersectionIsSubsetOfBoth'(A: set, B: set, C: set)
+	requires pre: C == SetIntersection(A, B) // == A*B
+	ensures IsSubset(C, A) // Post1: C <= A
+	ensures IsSubset(C, B) // Post2: C <= B
+{
+	//reveal pre; // we prefer not to reveal the precondition too early, but rather only where needed,
+	// in order to demonstrate our understanding
+
+	// Post1:
+	assert IsSubset(C, A) by {
+		assert forall n :: n in C ==> n in A by {
+			//assert n in C; // the variable "n" is not defined here (it is out of scope)
+			forall m | m in C ensures m in A {
+				assert L1: m in C; //  we know this from the "|" of the forall statement above (the "such that" condition)
+				//assert m in A;// by { reveal pre; } //  this is what we need to show/demonstrate/prove
+				assert L2: m in A && m in B by { reveal pre,L1; } // and by the definition of SetIntersection
+				assert m in A by { reveal L2; AndImpliesBoth(m in A, m in B); } //  this is what we need to show/demonstrate/prove
+			}
+		}
+	}
+	// Post2 can be proved in a similar way
+	assert IsSubset(C, B) by { reveal pre; }
+}
+
+// this is obviously true, still we formulate it as another example for a lemma and the way it can be used
+// exercise: prove this using a truth table
+lemma AndImpliesBoth(P: bool, Q: bool)
+	ensures P && Q ==> P
+	ensures P && Q ==> Q
 {}
 
- 
+predicate IsStrictSubset(A: set, B: set) // "<" ("הכלה ממש")
+{
+	IsSubset(A, B) &&
+	(exists m :: m in B && m !in A)
+}
+
+// could be written also this way:
+predicate IsStrictSubset2(A: set, B: set) // "<" ("הכלה ממש")
+{
+	IsSubset(A, B) &&
+	SetDifference(B, A) != {} 
+}
+
+// could also be written also this way:
+predicate IsStrictSubset3(A: set, B: set)
+{
+	IsSubset(A, B) &&
+	|SetDifference(B, A)| != 0 
+}
+
+// and could also be written also this way:
+predicate IsStrictSubset4(A: set, B: set)
+{
+	IsSubset(A, B) &&
+	|A| < |B| 
+}
+
+// or this way:
+predicate IsStrictSubset5(A: set, B: set)
+{
+	IsSubset(A, B) &&
+	A != B // how to prove equality (or inequality) of two sets we will learn next week
+}
+
+// exercise: try to prove, or find a problem in the definition
+lemma {:verify false} EquivalentDefinitionsOfStrictSubset(A: set, B: set)
+	ensures IsStrictSubset(A, B) == IsStrictSubset2(A, B) == IsStrictSubset3(A, B) == IsStrictSubset4(A, B)
+{}
+
+lemma {:verify true} TransitivityOfSetInclusion(A: set, B: set, C: set)
+	requires pre1: IsSubset(A, B)
+	requires pre2: IsSubset(B, C)
+	ensures IsSubset(A, C)
+{
+	assert forall n :: n in A ==> n in C by { // in the future we will not write this assertion
+		forall m | m in A ensures m in C {
+			assert MemberOfA: m in A; //  we know this from the "|" of the forall statement above (the "such that" condition)
+			//assert m in C; //  this is what we need to show/demonstrate/prove
+			assert MemberOfB: m in B by { reveal MemberOfA,pre1; } // and by the definition of IsSubset
+			assert MemberOfC: m in C by { reveal MemberOfB,pre2; } // and again by the definition of IsSubset
+			reveal MemberOfC; // could skip this reveal by not providing a label to the assertion above
+		}
+	}
+}
+
+// whenever the intersection is empty we say the sets are disjoint (זרות)
+predicate DisjointSets(A: set, B: set) { SetIntersection(A, B) == {} }
+
+method M3a()
+{
+    assert {1,3,5} + {2,4,6} == {1,2,3,4,5,6};
+    assert {1,3,5} * {2,4,6} == {};
+    assert DisjointSets({1,3,5}, {2,4,6});
+    assert SetIntersection({1,3,4,5}, {2,4,6}) == {4}; // a set with one element is known as a singleton ("יחידון")
+    assert !DisjointSets({1,3,4,5}, {2,4,6}) by { assert 4 in {1,3,4,5} && 4 in {2,4,6}; } // the intersection is not empty: it is the singleton {4}
+}
+
+lemma SubsetsInDafny(A: set, B: set)
+    ensures A<=B <==> IsSubset(A, B)
+    ensures A>=B <==> IsSubset(B, A) // we can also say that A is a superset of B
+{}
+
+// two general properties: each set has the empty set and the set itself as subsets
+lemma EmptySubset(A: set)
+    ensures IsSubset({}, A)
+{}
+
+lemma SelfSubset(A: set)
+    ensures IsSubset(A, A)
+{}
+
+lemma NotSelfStrictSubset(A: set)
+    ensures !IsStrictSubset(A, A)
+{}
+
+predicate IsSuperset(A: iset, B: iset)
+{
+    forall n :: n in B ==> n in A // same as "A >= B"
+}
+
+// the union is always a superset of both sets
+lemma UnionIsSuperset(A: iset, B: iset)
+    ensures IsSuperset(SetUnion(A, B), A)
+    ensures IsSuperset(SetUnion(A, B), B)
+{} // Exercise: prove this by choosing an element and following the definition (of set-union this time)
+
+// example of negation of forall:
+lemma {:verify false} DeMorganOfForall(A: set<int>)
+	ensures !(forall x :: x in A <==> x%2 == 0) <==> (exists y :: y in A && y%2 != 0)
+{}
