tutorial03.dfy
@@ -1,0 +1,59 @@
+/*
+	tutorial 3: truth tables + first proofs with "forall ... ensures"
+*/
+
+/*
+
+A questions from last year's exam:
+
+בהינתן הנוסחה
+(p ==> (q && r)) <==> ((p ==> q) || (p ==> r))
+בכמה מתוך 8 השורות בטבלת האמת של נוסחה זו הערך הינו True ?
+
+ p  q  r  "q && r"  "p ==> (q && r)"  "p ==> q"  "p ==> r"   "(p ==> q) || (p ==> r)"    "(p ==> (q && r)) <==> ((p ==> q) || (p ==> r))"
+ F  F  F  F         T                 T          T           T                           T
+ F  F  T  F         T                 T          T           T                           T
+ F  T  F  F         T                 T          T           T                           T
+ F  T  T  T         T                 T          T           T                           T
+ T  F  F  F         F                 F          F           F                           T
+ T  F  T  F         F                 F          T           T                           F
+ T  T  F  F         F                 T          F           T                           F
+ T  T  T  T         T                 T          T           T                           T
+
+תשובה: 6
+
+*/
+
+include "lecture03.dfy"
+
+lemma TheEmptySetIsASubsetOfAnySet<T>(A: set<T>)
+    ensures IsSubset({}, A)
+{
+	forall n | n in {} ensures n in A {
+		assert L1: n in {}; // by the "|" above
+		assert L2: n !in {} by { TheEmptySetIsIndeedEmpty<T>(); }
+		// we reached a contradiction!
+		assert P: false by { reveal L1,L2; }
+		assert Q: false ==> n in A; // since false implies anything (for any P, "false ==> P")
+		assert n in A by { reveal P,Q; ModusPonens(false, n in A); } // let's return to that next week!
+	}
+}
+
+lemma TheEmptySetIsIndeedEmpty<T>()
+	ensures forall s: set<T>, n: T :: s == {} ==> n !in s
+{}
+
+lemma ModusPonens(P: bool, Q: bool)
+	requires P ==> Q
+	requires P
+	ensures Q
+{}
+
+lemma SelfSubset'(A: set)
+    ensures IsSubset(A, A)
+{
+	forall n | n in A ensures n in A {
+		assert L1: n in A; // by the "|" above
+		assert n in A by { reveal L1; }
+	}
+}
